generic version of sim

dimsum/iris/expr.v
@@ -26,197 +26,212 @@ Global Arguments mtrans {_ _} _.
 Global Arguments mexpr_rel {_ _} _ _ _.
 Global Arguments mstate_interp {_ _} _ _.
 
-(** * [sim_tgt_expr] *)
-Definition sim_tgt_expr_raw {EV Σ Λ} `{!dimsumGS Σ}
-  (e : mexpr Λ) (os : option (mstate Λ)) (Π : option EV → ((m_state Λ → iProp Σ) → iProp Σ) → iProp Σ) : iProp Σ :=
+(** * [sim_gen_expr] *)
+Definition sim_gen_expr_raw {EV Σ Λ} `{!dimsumGS Σ}
+  (ts : tgt_src) (e : mexpr Λ) (os : option (mstate Λ)) (Π : option EV → m_state Λ → iProp Σ) : iProp Σ :=
   (∀ σ, ⌜mexpr_rel Λ σ e⌝ -∗ ord_later_ctx -∗ mstate_interp Λ σ os -∗
-    σ ≈{ Λ }≈>ₜ Π)%I.
+    σ ≈{ ts, Λ }≈> Π)%I.
 
-Notation "'TGT' e @ ? os [{ Π }]" := (sim_tgt_expr_raw e os Π%I) (at level 70, Π at level 200,
+Notation "'WP{' ts '}' e @ ? os [{ Π }]" := (sim_gen_expr_raw ts e os Π%I) (at level 70, Π at level 200,
+  format "'[hv' 'WP{' ts '}'  e  '/' @  ?  os  [{  '[ ' Π  ']' }] ']'") : bi_scope.
+Notation "'WP{' ts '}' e @ s [{ Π }]" := (sim_gen_expr_raw ts e (Some s) Π%I) (at level 70, Π at level 200,
+  format "'[hv' 'WP{' ts '}'  e  '/' @  s  [{  '[ ' Π  ']' }] ']'") : bi_scope.
+Notation "'WP{' ts '}' e [{ Π }]" := (sim_gen_expr_raw ts e None Π%I) (at level 70, Π at level 200,
+  format "'[hv' 'WP{' ts '}'  e  '/' [{  '[ ' Π  ']' }] ']'") : bi_scope.
+
+Notation "'TGT' e @ ? os [{ Π }]" := (sim_gen_expr_raw Tgt e os Π%I) (at level 70, Π at level 200,
   format "'[hv' 'TGT'  e  '/' @  ?  os  [{  '[ ' Π  ']' }] ']'") : bi_scope.
-Notation "'TGT' e @ s [{ Π }]" := (sim_tgt_expr_raw e (Some s) Π%I) (at level 70, Π at level 200,
+Notation "'TGT' e @ s [{ Π }]" := (sim_gen_expr_raw Tgt e (Some s) Π%I) (at level 70, Π at level 200,
   format "'[hv' 'TGT'  e  '/' @  s  [{  '[ ' Π  ']' }] ']'") : bi_scope.
-Notation "'TGT' e [{ Π }]" := (sim_tgt_expr_raw e None Π%I) (at level 70, Π at level 200,
+Notation "'TGT' e [{ Π }]" := (sim_gen_expr_raw Tgt e None Π%I) (at level 70, Π at level 200,
   format "'[hv' 'TGT'  e  '/' [{  '[ ' Π  ']' }] ']'") : bi_scope.
 
-Definition sim_tgt_expr {EV Σ Λ} `{!dimsumGS Σ}
-  (e : mexpr Λ) (os : option (mstate Λ)) (Π : option EV → ((m_state Λ → iProp Σ) → iProp Σ) → iProp Σ)
-  (Φ : mexpr Λ → option (mstate Λ) → (option EV → ((m_state Λ → iProp Σ) → iProp Σ) → iProp Σ) → iProp Σ): iProp Σ :=
-  ∀ K, (∀ e' os' Π', Φ e' os' Π' -∗ TGT mfill Λ K e' @ ? os' [{ Π' }]) -∗ TGT mfill Λ K e @ ? os [{ Π }].
+Notation "'SRC' e @ ? os [{ Π }]" := (sim_gen_expr_raw Src e os Π%I) (at level 70, Π at level 200,
+  format "'[hv' 'SRC'  e  '/' @  ?  os  [{  '[ ' Π  ']' }] ']'") : bi_scope.
+Notation "'SRC' e @ s [{ Π }]" := (sim_gen_expr_raw Src e (Some s) Π%I) (at level 70, Π at level 200,
+  format "'[hv' 'SRC'  e  '/' @  s  [{  '[ ' Π  ']' }] ']'") : bi_scope.
+Notation "'SRC' e [{ Π }]" := (sim_gen_expr_raw Src e None Π%I) (at level 70, Π at level 200,
+  format "'[hv' 'SRC'  e  '/' [{  '[ ' Π  ']' }] ']'") : bi_scope.
 
-Notation "'TGT' e @ ? os [{ Π }] {{ Φ } }" := (sim_tgt_expr e os Π%I Φ%I)
+Definition sim_gen_expr {EV Σ Λ} `{!dimsumGS Σ}
+  (ts : tgt_src) (e : mexpr Λ) (os : option (mstate Λ)) (Π : option EV → m_state Λ → iProp Σ)
+  (Φ : mexpr Λ → option (mstate Λ) → (option EV → m_state Λ → iProp Σ) → iProp Σ): iProp Σ :=
+  ∀ K, (∀ e' os' Π', Φ e' os' Π' -∗ WP{ts} mfill Λ K e' @ ? os' [{ Π' }]) -∗ WP{ts} mfill Λ K e @ ? os [{ Π }].
+
+Notation "'WP{' ts '}' e @ ? os [{ Π }] {{ Φ } }" := (sim_gen_expr ts e os Π%I Φ%I)
   (at level 70, Π, Φ at level 200, only parsing) : bi_scope.
-Notation "'TGT' e @ s [{ Π }] {{ Φ } }" := (sim_tgt_expr e (Some s) Π%I Φ%I)
+Notation "'WP{' ts '}' e @ s [{ Π }] {{ Φ } }" := (sim_gen_expr ts e (Some s) Π%I Φ%I)
   (at level 70, Π, Φ at level 200, only parsing) : bi_scope.
-Notation "'TGT' e [{ Π }] {{ Φ } }" := (sim_tgt_expr e None Π%I Φ%I)
+Notation "'WP{' ts '}' e [{ Π }] {{ Φ } }" := (sim_gen_expr ts e None Π%I Φ%I)
   (at level 70, Π, Φ at level 200, only parsing) : bi_scope.
 
-Notation "'TGT' e @ ? os [{ Π }] {{ e' , os' , Π' , Φ } }" := (sim_tgt_expr e os Π%I (λ e' os' Π', Φ%I))
+Notation "'WP{' ts '}' e @ ? os [{ Π }] {{ e' , os' , Π' , Φ } }" := (sim_gen_expr ts e os Π%I (λ e' os' Π', Φ%I))
+  (at level 70, Π, Φ at level 200,
+    format "'[hv' 'WP{' ts '}'  e  '/' @  ?  os  [{  '[ ' Π  ']' }]  {{  '[ ' e' ,  os' ,  Π' ,  '/' Φ  ']' } } ']'") : bi_scope.
+Notation "'WP{' ts '}' e @ s [{ Π }] {{ e' , os' , Π' , Φ } }" := (sim_gen_expr ts e (Some s) Π%I (λ e' os' Π', Φ%I))
+  (at level 70, Π, Φ at level 200,
+    format "'[hv' 'WP{' ts '}'  e  '/' @  s  [{  '[ ' Π  ']' }]  {{  '[ ' e' ,  os' ,  Π' ,  '/' Φ  ']' } } ']'") : bi_scope.
+Notation "'WP{' ts '}' e [{ Π }] {{ e' , os' , Π' , Φ } }" := (sim_gen_expr ts e None Π%I (λ e' os' Π', Φ%I))
+  (at level 70, Π, Φ at level 200,
+    format "'[hv' 'WP{' ts '}'  e  '/' [{  '[ ' Π  ']' }]  {{  '[ ' e' ,  os' ,  Π' ,  '/' Φ  ']' } } ']'") : bi_scope.
+
+Notation "'TGT' e @ ? os [{ Π }] {{ Φ } }" := (sim_gen_expr Tgt e os Π%I Φ%I)
+  (at level 70, Π, Φ at level 200, only parsing) : bi_scope.
+Notation "'TGT' e @ s [{ Π }] {{ Φ } }" := (sim_gen_expr Tgt e (Some s) Π%I Φ%I)
+  (at level 70, Π, Φ at level 200, only parsing) : bi_scope.
+Notation "'TGT' e [{ Π }] {{ Φ } }" := (sim_gen_expr Tgt e None Π%I Φ%I)
+  (at level 70, Π, Φ at level 200, only parsing) : bi_scope.
+
+Notation "'TGT' e @ ? os [{ Π }] {{ e' , os' , Π' , Φ } }" := (sim_gen_expr Tgt e os Π%I (λ e' os' Π', Φ%I))
   (at level 70, Π, Φ at level 200,
     format "'[hv' 'TGT'  e  '/' @  ?  os  [{  '[ ' Π  ']' }]  {{  '[ ' e' ,  os' ,  Π' ,  '/' Φ  ']' } } ']'") : bi_scope.
-Notation "'TGT' e @ s [{ Π }] {{ e' , os' , Π' , Φ } }" := (sim_tgt_expr e (Some s) Π%I (λ e' os' Π', Φ%I))
+Notation "'TGT' e @ s [{ Π }] {{ e' , os' , Π' , Φ } }" := (sim_gen_expr Tgt e (Some s) Π%I (λ e' os' Π', Φ%I))
   (at level 70, Π, Φ at level 200,
     format "'[hv' 'TGT'  e  '/' @  s  [{  '[ ' Π  ']' }]  {{  '[ ' e' ,  os' ,  Π' ,  '/' Φ  ']' } } ']'") : bi_scope.
-Notation "'TGT' e [{ Π }] {{ e' , os' , Π' , Φ } }" := (sim_tgt_expr e None Π%I (λ e' os' Π', Φ%I))
+Notation "'TGT' e [{ Π }] {{ e' , os' , Π' , Φ } }" := (sim_gen_expr Tgt e None Π%I (λ e' os' Π', Φ%I))
   (at level 70, Π, Φ at level 200,
     format "'[hv' 'TGT'  e  '/' [{  '[ ' Π  ']' }]  {{  '[ ' e' ,  os' ,  Π' ,  '/' Φ  ']' } } ']'") : bi_scope.
 
-Section sim_tgt.
+Notation "'SRC' e @ ? os [{ Π }] {{ Φ } }" := (sim_gen_expr Src e os Π%I Φ%I)
+  (at level 70, Π, Φ at level 200, only parsing) : bi_scope.
+Notation "'SRC' e @ s [{ Π }] {{ Φ } }" := (sim_gen_expr Src e (Some s) Π%I Φ%I)
+  (at level 70, Π, Φ at level 200, only parsing) : bi_scope.
+Notation "'SRC' e [{ Π }] {{ Φ } }" := (sim_gen_expr Src e None Π%I Φ%I)
+  (at level 70, Π, Φ at level 200, only parsing) : bi_scope.
+
+Notation "'SRC' e @ ? os [{ Π }] {{ e' , os' , Π' , Φ } }" := (sim_gen_expr Src e os Π%I (λ e' os' Π', Φ%I)) (at level 70, Π, Φ at level 200,
+  format "'[hv' 'SRC'  e  '/' @  ?  os  [{  '[ ' Π  ']' }]  {{  '[ ' e' ,  os' ,  Π' ,  '/' Φ  ']' } } ']'") : bi_scope.
+Notation "'SRC' e @ s [{ Π }] {{ e' , os' , Π' , Φ } }" := (sim_gen_expr Src e (Some s) Π%I (λ e' os' Π', Φ%I)) (at level 70, Π, Φ at level 200,
+  format "'[hv' 'SRC'  e  '/' @  s  [{  '[ ' Π  ']' }]  {{  '[ ' e' ,  os' ,  Π' ,  '/' Φ  ']' } } ']'") : bi_scope.
+Notation "'SRC' e [{ Π }] {{ e' , os' , Π' , Φ } }" := (sim_gen_expr Src e None Π%I (λ e' os' Π', Φ%I)) (at level 70, Π, Φ at level 200,
+  format "'[hv' 'SRC'  e  '/' [{  '[ ' Π  ']' }]  {{  '[ ' e' ,  os' ,  Π' ,  '/' Φ  ']' } } ']'") : bi_scope.
+
+Section sim_gen.
 Context {EV} {Σ} {Λ : mod_lang EV Σ} `{!dimsumGS Σ}.
+Context (ts : tgt_src).
 Implicit Types (e : mexpr Λ).
 
-Lemma sim_tgt_expr_raw_step e Π os :
-  (∀ σ κ Pσ, ⌜mexpr_rel Λ σ e⌝ -∗ ⌜Λ.(m_step) σ κ Pσ⌝ -∗ mstate_interp Λ σ os ={∅}=∗ ▷ₒ
-      (Π κ (λ P', ∃ σ', ⌜Pσ σ'⌝ ∗ P' σ') ∨
-         ∃ os' σ' e', ⌜κ = None⌝ ∗ ⌜Pσ σ'⌝ ∗ ⌜mexpr_rel Λ σ' e'⌝ ∗ mstate_interp Λ σ' os' ∗ TGT e' @ ? os' [{ Π }])) -∗
-  TGT e @ ? os [{ Π }].
-Proof.
-  iIntros "HΠ" (σ ?) "#??".
-  iApply sim_tgt_step. iIntros (???). iMod ("HΠ" with "[//] [//] [$]") as "Hsim". do 2 iModIntro.
-  iDestruct "Hsim" as "[$|(%&%&%&%&%&%&?&Hsim)]". iRight. iExists _. iSplit; [done|]. iSplit; [done|].
-  by iApply "Hsim".
-Qed.
-
-Lemma sim_tgt_expr_raw_elim e Π σ os :
+Lemma sim_gen_expr_raw_elim e Π σ os :
   mexpr_rel Λ σ e →
   mstate_interp Λ σ os -∗
-  TGT e @ ? os [{ Π }] -∗
-  σ ≈{Λ}≈>ₜ Π.
-Proof. iIntros (?) "Hσ He". iApply sim_tgt_ctx. iIntros "#?". by iApply "He". Qed.
+  WP{ts} e @ ? os [{ Π }] -∗
+  σ ≈{ts, Λ}≈> Π.
+Proof. iIntros (?) "Hσ He". iApply sim_gen_ctx. iIntros "#?". by iApply "He". Qed.
 
-Lemma sim_tgt_expr_ctx e Π Φ os :
-  (ord_later_ctx -∗ TGT e @ ? os [{ Π }] {{ Φ }}) -∗
-  TGT e @ ? os [{ Π }] {{ Φ }}.
+Lemma sim_gen_expr_ctx e Π Φ os :
+  (ord_later_ctx -∗ WP{ts} e @ ? os [{ Π }] {{ Φ }}) -∗
+  WP{ts} e @ ? os [{ Π }] {{ Φ }}.
 Proof.
   iIntros "Hsim" (?) "HΦ". iIntros (??) "#?". iApply ("Hsim" with "[$] [$] [//] [$]").
 Qed.
 
-Lemma fupd_sim_tgt_expr e Π Φ os :
-  (|={∅}=> TGT e @ ? os [{ Π }] {{ Φ }}) -∗
-  TGT e @ ? os [{ Π }] {{ Φ }}.
+Lemma fupd_sim_gen_expr e Π Φ os :
+  (|={∅}=> WP{ts} e @ ? os [{ Π }] {{ Φ }}) -∗
+  WP{ts} e @ ? os [{ Π }] {{ Φ }}.
 Proof.
-  iIntros "Hsim" (?) "HΦ". iIntros (??) "#??". iApply fupd_sim_tgt. iApply ("Hsim" with "[$] [//] [//] [$]").
+  iIntros "Hsim" (?) "HΦ". iIntros (??) "#??". iApply fupd_sim_gen. iApply ("Hsim" with "[$] [//] [//] [$]").
 Qed.
 
-Lemma sim_tgt_expr_bi_mono e Π Φ os :
-  (TGT e @ ? os [{ λ κ, bi_mono1 (Π κ) }] {{ Φ }}) -∗
-  TGT e @ ? os [{ Π }] {{ Φ }}.
-Proof.
-  iIntros "Hsim" (?) "HΦ". iIntros (??) "#??". iApply sim_tgt_bi_mono1.
-  iApply ("Hsim" with "[$] [//] [//] [$]").
-Qed.
-
-Lemma sim_tgt_expr_bind K e Π Φ os :
-  TGT e @ ? os [{ Π }] {{ e', os', Π', TGT mfill Λ K e' @ ? os' [{ Π' }] {{ Φ }} }} -∗
-  TGT mfill Λ K e @ ? os [{ Π }] {{ Φ }}.
+Lemma sim_gen_expr_bind K e Π Φ os :
+  WP{ts} e @ ? os [{ Π }] {{ e', os', Π', WP{ts} mfill Λ K e' @ ? os' [{ Π' }] {{ Φ }} }} -∗
+  WP{ts} mfill Λ K e @ ? os [{ Π }] {{ Φ }}.
 Proof.
   iIntros "Hsim" (?) "HΦ". rewrite mfill_comp. iApply "Hsim".
   iIntros (???) "Htgt". rewrite -mfill_comp. by iApply "Htgt".
 Qed.
 
-Lemma sim_tgt_expr_wand1 e Π Π' Φ os :
-  TGT e @ ? os [{ Π' }] {{ Φ }} -∗
+Lemma sim_gen_expr_wand1 e Π Π' Φ os :
+  WP{ts} e @ ? os [{ Π' }] {{ Φ }} -∗
   (∀ κ P, Π' κ P -∗ Π κ P) -∗
-  TGT e @ ? os [{ Π }] {{ Φ }}.
+  WP{ts} e @ ? os [{ Π }] {{ Φ }}.
 Proof.
   iIntros "Hsim Hwand" (?) "HΦ".
   iIntros (??) "#? Hσ".
-  iApply (sim_tgt_wand with "[Hσ HΦ Hsim] Hwand").
+  iApply (sim_gen_wand with "[Hσ HΦ Hsim] Hwand").
   iApply ("Hsim" with "[$] [//] [$] [$]").
 Qed.
 
-Lemma sim_tgt_expr_wand e Π Φ Φ' os :
-  TGT e @ ? os [{ Π }] {{ Φ' }} -∗
+Lemma sim_gen_expr_wand e Π Φ Φ' os :
+  WP{ts} e @ ? os [{ Π }] {{ Φ' }} -∗
   (∀ e' os' Π', Φ' e' os' Π' -∗ Φ e' os' Π') -∗
-  TGT e @ ? os [{ Π }] {{ Φ }}.
+  WP{ts} e @ ? os [{ Π }] {{ Φ }}.
 Proof. iIntros "Hsim Hwand" (?) "HΦ". iApply "Hsim". iIntros (???) "Hsim". iApply "HΦ". by iApply "Hwand". Qed.
 
-Lemma sim_tgt_expr_stop1 e Π Φ os :
-  (∀ σ, σ ⤇ₜ (λ Π', TGT e @ ? os [{ Π' }] {{ Φ }}) -∗ Π None (λ P, P σ)) -∗
-  TGT e @ ? os [{ Π }] {{ Φ }}.
+Lemma sim_gen_expr_stop1 e Π Φ os :
+  (∀ σ, σ ⤇{ts} (λ Π', WP{ts} e @ ? os [{ Π' }] {{ Φ }}) -∗ Π None σ) -∗
+  WP{ts} e @ ? os [{ Π }] {{ Φ }}.
 Proof.
   iIntros "HΦ" (?) "HF". iIntros (??) "??".
-  iApply sim_tgt_stop. iApply "HΦ". iIntros (?) "Hsim".
+  iApply sim_gen_stop. iApply "HΦ". iIntros (?) "Hsim".
   iApply ("Hsim" with "[$] [//] [$] [$]").
 Qed.
 
-Lemma sim_tgt_expr_stop2 e Π Φ os :
-  Φ e os Π -∗ TGT e @ ? os [{ Π }] {{ Φ }}.
+Lemma sim_gen_expr_stop2 e Π Φ os :
+  Φ e os Π -∗ WP{ts} e @ ? os [{ Π }] {{ Φ }}.
 Proof. iIntros "HΦ" (?) "HF". by iApply "HF". Qed.
 
-Lemma sim_tgt_expr_elim os K e Π σ :
+Lemma sim_gen_expr_elim os K e Π σ :
   mexpr_rel Λ σ (mfill Λ K e) →
   mstate_interp Λ σ os -∗
-  TGT e @ ? os [{ Π }] {{ _, _, _, False }} -∗
-  σ ≈{Λ}≈>ₜ Π.
+  WP{ts} e @ ? os [{ Π }] {{ _, _, _, False }} -∗
+  σ ≈{ts, Λ}≈> Π.
 Proof.
-  iIntros (?) "Hσ He". iApply (sim_tgt_expr_raw_elim with "[$]"); [done|].
+  iIntros (?) "Hσ He". iApply (sim_gen_expr_raw_elim with "[$]"); [done|].
   iApply "He". by iIntros (???) "?".
+Qed.
+End sim_gen.
+
+(** * [sim_tgt_expr] *)
+Section sim_tgt.
+Context {EV} {Σ} {Λ : mod_lang EV Σ} `{!dimsumGS Σ}.
+Implicit Types (e : mexpr Λ).
+
+Lemma sim_tgt_expr_raw_step e Π os :
+  (∀ σ κ Pσ, ⌜mexpr_rel Λ σ e⌝ -∗ ⌜Λ.(m_step) σ κ Pσ⌝ -∗ mstate_interp Λ σ os ={∅}=∗ ∃ σ', ⌜Pσ σ'⌝ ∗ ▷ₒ
+      (Π κ σ' ∨
+       ∃ os' e', ⌜κ = None⌝ ∗ ⌜mexpr_rel Λ σ' e'⌝ ∗
+                  mstate_interp Λ σ' os' ∗ TGT e' @ ? os' [{ Π }])) -∗
+  TGT e @ ? os [{ Π }].
+Proof.
+  iIntros "HΠ" (σ ?) "#??".
+  iApply sim_gen_step => /=. iIntros ([??]?). iMod ("HΠ" with "[//] [//] [$]") as (??) "Hsim".
+  iModIntro. iExists _. iSplit; [done|]. do 2 iModIntro => /=.
+  iDestruct "Hsim" as "[$|(%&%&%&%&?&Hsim)]". iRight. iSplit; [done|]. by iApply "Hsim".
 Qed.
 
 Lemma sim_tgt_expr_step_None e Π Φ os :
-  (∀ K σ κ Pσ, ⌜mexpr_rel Λ σ (mfill Λ K e)⌝ -∗ ⌜Λ.(m_step) σ κ Pσ⌝ -∗ mstate_interp Λ σ os ={∅}=∗ ▷ₒ
-      (∃ os' σ' e', ⌜κ = None⌝ ∗ ⌜Pσ σ'⌝ ∗ ⌜mexpr_rel Λ σ' (mfill Λ K e')⌝ ∗ mstate_interp Λ σ' os' ∗ TGT e' @ ? os' [{ Π }] {{Φ}})) -∗
+  (∀ K σ κ Pσ, ⌜mexpr_rel Λ σ (mfill Λ K e)⌝ -∗ ⌜Λ.(m_step) σ κ Pσ⌝ -∗ mstate_interp Λ σ os ={∅}=∗
+      ∃ σ', ⌜Pσ σ'⌝ ∗
+      ▷ₒ (∃ os' e', ⌜κ = None⌝ ∗ ⌜mexpr_rel Λ σ' (mfill Λ K e')⌝ ∗ mstate_interp Λ σ' os' ∗ TGT e' @ ? os' [{ Π }] {{Φ}})) -∗
   TGT e @ ? os [{ Π }] {{ Φ }}.
 Proof.
   iIntros "Hs" (?) "HΦ". iApply sim_tgt_expr_raw_step. iIntros (?????) "?".
-  iMod ("Hs" with "[//] [//] [$]") as "Hs". do 2 iModIntro. iRight.
-  iDestruct "Hs" as (??????) "[? Hsim]". iExists _, _, _. iSplit; [done|]. iSplit; [done|]. iSplit; [done|].
+  iMod ("Hs" with "[//] [//] [$]") as (??)"Hs". iModIntro. iExists _. iSplit; [done|].
+  iModIntro. iDestruct "Hs" as (????) "[? Hsim]". iRight.
+  iExists _, _. iSplit; [done|]. iSplit; [done|].
   iFrame. by iApply "Hsim".
 Qed.
 
 Lemma sim_tgt_expr_step e Φ Π os :
-  (∀ K σ κ Pσ, ⌜mexpr_rel Λ σ (mfill Λ K e)⌝ -∗ ⌜m_step Λ σ κ Pσ⌝ -∗ mstate_interp Λ σ os ={∅}=∗ ▷ₒ
-     Π κ (λ P, ∃ σ', ⌜Pσ σ'⌝ ∗
-       ((∀ os' e',
+  (∀ K σ κ Pσ, ⌜mexpr_rel Λ σ (mfill Λ K e)⌝ -∗ ⌜m_step Λ σ κ Pσ⌝ -∗ mstate_interp Λ σ os ={∅}=∗
+    ∃ σ', ⌜Pσ σ'⌝ ∗ ((∀ os' e',
            ⌜mexpr_rel Λ σ' (mfill Λ K e')⌝ -∗
            mstate_interp Λ σ' os' -∗
            σ' ⤇ₜ λ Π', TGT e' @ ? os' [{ Π' }] {{ Φ }}) -∗
-          P σ'))) -∗
+           ▷ₒ Π κ σ')) -∗
   TGT e @ ? os [{ Π }] {{ Φ }}.
 Proof.
   iIntros "Hsim" (?). iIntros "HΦ" (??) "#? Hσ".
-  iApply sim_tgt_bi_mono1. iApply sim_tgt_step_end. iIntros (???). iMod ("Hsim" with "[//] [//] [$]") as "Hsim".
-  do 2 iModIntro. iApply (bi_mono1_intro with "Hsim"). iIntros (?) "[% [% Hsim]]".
-  iExists _. iSplit; [done|]. iApply "Hsim".
-  iIntros (???) "?". iIntros (?) "Hsim". iApply (sim_tgt_expr_raw_elim with "[$]"); [done|].
+  iApply sim_gen_step_end. iIntros (??). iMod ("Hsim" with "[//] [//] [$]") as (??) "Hsim".
+  iModIntro. iExists _. iSplit; [done|].
+  iSpecialize ("Hsim" with "[-]"); [|by do 2 iModIntro].
+  iIntros (???) "?". iIntros (?) "Hsim". iApply (sim_gen_expr_raw_elim with "[$]"); [done|].
   by iApply "Hsim".
 Qed.
 
 End sim_tgt.
 
 (** * [sim_src_expr] *)
-Definition sim_src_expr_raw {EV Σ Λ} `{!dimsumGS Σ}
-  (e : mexpr Λ) (os : option (mstate Λ)) (Π : option EV → m_state Λ → iProp Σ) : iProp Σ :=
-  (∀ σ, ⌜mexpr_rel Λ σ e⌝ -∗ ord_later_ctx -∗ mstate_interp Λ σ os -∗
-    σ ≈{ Λ }≈>ₛ Π)%I.
-
-Notation "'SRC' e @ ? os [{ Π }]" := (sim_src_expr_raw e os Π%I) (at level 70, Π at level 200,
-  format "'[hv' 'SRC'  e  '/' @  ?  os  [{  '[ ' Π  ']' }] ']'") : bi_scope.
-Notation "'SRC' e @ s [{ Π }]" := (sim_src_expr_raw e (Some s) Π%I) (at level 70, Π at level 200,
-  format "'[hv' 'SRC'  e  '/' @  s  [{  '[ ' Π  ']' }] ']'") : bi_scope.
-Notation "'SRC' e [{ Π }]" := (sim_src_expr_raw e None Π%I) (at level 70, Π at level 200,
-  format "'[hv' 'SRC'  e  '/' [{  '[ ' Π  ']' }] ']'") : bi_scope.
-
-Definition sim_src_expr {EV Σ Λ} `{!dimsumGS Σ}
-  (e : mexpr Λ) (os : option (mstate Λ)) (Π : option EV → m_state Λ → iProp Σ)
-  (Φ : mexpr Λ → option (mstate Λ) → (option EV → m_state Λ → iProp Σ) → iProp Σ): iProp Σ :=
-  ∀ K, (∀ e' os' Π', Φ e' os' Π' -∗ SRC mfill Λ K e' @ ? os' [{ Π' }]) -∗ SRC mfill Λ K e @ ? os [{ Π }].
-
-Notation "'SRC' e @ ? os [{ Π }] {{ Φ } }" := (sim_src_expr e os Π%I Φ%I)
-  (at level 70, Π, Φ at level 200, only parsing) : bi_scope.
-Notation "'SRC' e @ s [{ Π }] {{ Φ } }" := (sim_src_expr e (Some s) Π%I Φ%I)
-  (at level 70, Π, Φ at level 200, only parsing) : bi_scope.
-Notation "'SRC' e [{ Π }] {{ Φ } }" := (sim_src_expr e None Π%I Φ%I)
-  (at level 70, Π, Φ at level 200, only parsing) : bi_scope.
-
-Notation "'SRC' e @ ? os [{ Π }] {{ e' , os' , Π' , Φ } }" := (sim_src_expr e os Π%I (λ e' os' Π', Φ%I)) (at level 70, Π, Φ at level 200,
-  format "'[hv' 'SRC'  e  '/' @  ?  os  [{  '[ ' Π  ']' }]  {{  '[ ' e' ,  os' ,  Π' ,  '/' Φ  ']' } } ']'") : bi_scope.
-Notation "'SRC' e @ s [{ Π }] {{ e' , os' , Π' , Φ } }" := (sim_src_expr e (Some s) Π%I (λ e' os' Π', Φ%I)) (at level 70, Π, Φ at level 200,
-  format "'[hv' 'SRC'  e  '/' @  s  [{  '[ ' Π  ']' }]  {{  '[ ' e' ,  os' ,  Π' ,  '/' Φ  ']' } } ']'") : bi_scope.
-Notation "'SRC' e [{ Π }] {{ e' , os' , Π' , Φ } }" := (sim_src_expr e None Π%I (λ e' os' Π', Φ%I)) (at level 70, Π, Φ at level 200,
-  format "'[hv' 'SRC'  e  '/' [{  '[ ' Π  ']' }]  {{  '[ ' e' ,  os' ,  Π' ,  '/' Φ  ']' } } ']'") : bi_scope.
-
 Section sim_src.
 Context {EV} {Σ} {Λ : mod_lang EV Σ} `{!dimsumGS Σ}.
 Implicit Types (e : mexpr Λ).
@@ -228,81 +243,12 @@ Lemma sim_src_expr_raw_step e Π os :
        ∃ os' e', ⌜mexpr_rel Λ σ' e'⌝ ∗ mstate_interp Λ σ' os' ∗ SRC e' @ ? os' [{ Π }]) -∗
   SRC e @ ? os [{ Π }].
 Proof.
-  iIntros "HΠ" (σ ?) "#??". iApply fupd_sim_src.
+  iIntros "HΠ" (σ ?) "#??". iApply fupd_sim_gen.
   iMod ("HΠ" with "[//] [$]") as (???) "HΠ". iModIntro.
-  iApply sim_src_step; [done..|]. iIntros (??).
-  iMod ("HΠ" with "[//]") as "HΠ". case_match; [done|]. iModIntro.
-  iDestruct ("HΠ") as (???) "[? Hsim]".
+  iApply sim_gen_step. iExists (_, _). iSplit; [done|]. iIntros "!>" (??).
+  iMod ("HΠ" with "[//]") as "HΠ". iModIntro. simpl. case_match; [iFrame|].
+  iRight. iSplit; [done|]. iDestruct ("HΠ") as (???) "[? Hsim]".
   by iApply "Hsim".
-Qed.
-
-Lemma sim_src_expr_raw_elim e Π σ os :
-  mexpr_rel Λ σ e →
-  mstate_interp Λ σ os -∗
-  SRC e @ ? os [{ Π }] -∗
-  σ ≈{Λ}≈>ₛ Π.
-Proof. iIntros (?) "Hσ He". iApply sim_src_ctx. iIntros "#?". by iApply "He". Qed.
-
-Lemma fupd_sim_src_expr e Π Φ os :
-  (|={∅}=> SRC e @ ? os [{ Π }] {{ Φ }}) -∗
-  SRC e @ ? os [{ Π }] {{ Φ }}.
-Proof.
-  iIntros "Hsim" (?) "HΦ". iIntros (??) "#??". iApply fupd_sim_src. iApply ("Hsim" with "[$] [//] [//] [$]").
-Qed.
-
-Lemma sim_src_expr_ctx e Π Φ os :
-  (ord_later_ctx -∗ SRC e @ ? os [{ Π }] {{ Φ }}) -∗
-  SRC e @ ? os [{ Π }] {{ Φ }}.
-Proof.
-  iIntros "Hsim" (?) "HΦ". iIntros (??) "#?". iApply ("Hsim" with "[$] [$] [//] [$]").
-Qed.
-
-Lemma sim_src_expr_bind e Π Φ K os :
-  SRC e @ ? os [{ Π }] {{ e', os', Π', SRC mfill Λ K e' @ ? os' [{ Π' }] {{ Φ }} }} -∗
-  SRC mfill Λ K e @ ? os [{ Π }] {{ Φ }}.
-Proof.
-  iIntros "Hsim" (?) "HΦ". rewrite mfill_comp. iApply "Hsim".
-  iIntros (???) "Htgt". rewrite -mfill_comp. by iApply "Htgt".
-Qed.
-
-Lemma sim_src_expr_wand1 e Π Π' Φ os :
-  SRC e @ ? os [{ Π' }] {{ Φ }} -∗
-  (∀ κ P, Π' κ P -∗ Π κ P) -∗
-  SRC e @ ? os [{ Π }] {{ Φ }}.
-Proof.
-  iIntros "Hsim Hwand" (?) "HΦ".
-  iIntros (??) "#? Hσ".
-  iApply (sim_src_wand with "[Hσ HΦ Hsim] Hwand").
-  iApply ("Hsim" with "[$] [//] [$] [$]").
-Qed.
-
-Lemma sim_src_expr_wand e Π Φ Φ' os :
-  SRC e @ ? os [{ Π }] {{ Φ' }} -∗
-  (∀ e' os' Π', Φ' e' os' Π' -∗ Φ e' os' Π') -∗
-  SRC e @ ? os [{ Π }] {{ Φ }}.
-Proof. iIntros "Hsim Hwand" (?) "HΦ". iApply "Hsim". iIntros (???) "Hsim". iApply "HΦ". by iApply "Hwand". Qed.
-
-Lemma sim_src_expr_stop1 e Π Φ os :
-  (∀ σ, σ ⤇ₛ (λ Π', SRC e @ ? os [{ Π' }] {{ Φ }}) -∗ Π None σ) -∗
-  SRC e @ ? os [{ Π }] {{ Φ }}.
-Proof.
-  iIntros "HΦ" (?) "HF". iIntros (??) "??".
-  iApply sim_src_stop. iApply "HΦ". iIntros (?) "Hsim".
-  iApply ("Hsim" with "[$] [//] [$] [$]").
-Qed.
-
-Lemma sim_src_expr_stop2 e Π Φ os :
-  Φ e os Π -∗ SRC e @ ? os [{ Π }] {{ Φ }}.
-Proof. iIntros "HΦ" (?) "HF". by iApply "HF". Qed.
-
-Lemma sim_src_expr_elim os e Π σ K :
-  mexpr_rel Λ σ (mfill Λ K e) →
-  mstate_interp Λ σ os -∗
-  SRC e @ ? os [{ Π }] {{ _, _, _, False }} -∗
-  σ ≈{Λ}≈>ₛ Π.
-Proof.
-  iIntros (?) "Hσ He". iApply (sim_src_expr_raw_elim with "[$]"); [done|].
-  iApply "He". by iIntros (???) "?".
 Qed.
 
 Lemma sim_src_expr_step_None e Π Φ os :
@@ -329,18 +275,18 @@ Lemma sim_src_expr_step e Φ Π os :
           Π κ' σ')) -∗
   SRC e @ ? os [{ Π }] {{ Φ }}.
 Proof.
-  iIntros "He" (?). iIntros "HΦ" (??) "#? Hσ". iApply fupd_sim_src.
+  iIntros "He" (?). iIntros "HΦ" (??) "#? Hσ". iApply fupd_sim_gen.
   iMod ("He" with "[//] [$]") as (???) "Hsim". iModIntro.
-  iApply sim_src_step_end; [done|]. iIntros (??). iMod ("Hsim" with "[//]") as "Hsim".
-  iModIntro. iApply "Hsim". iIntros (???) "?". iIntros (?) "Hsim".
-  iApply (sim_src_expr_raw_elim with "[$]"); [done|].
+  iApply sim_gen_step_end. iExists (_, _). iSplit; [done|].
+  iIntros "!>" (??). iMod ("Hsim" with "[//]") as "Hsim". iModIntro.
+  iApply "Hsim". iIntros (???) "?". iIntros (?) "Hsim".
+  iApply (sim_gen_expr_raw_elim with "[$]"); [done|].
   by iApply "Hsim".
 Qed.
-
 End sim_src.
 
-Global Typeclasses Opaque sim_tgt_expr sim_src_expr.
-Global Opaque sim_tgt_expr sim_src_expr.
+Global Typeclasses Opaque sim_gen_expr sim_gen_expr.
+Global Opaque sim_gen_expr sim_gen_expr.
 
 (* (** * [sim_expr_s] *) *)
 (* Definition sim_expr_s `{!dimsumGS EV Σ Λ_t Λ_s} (q : Qp) (e : mexpr Λ_s) : iProp Σ := *)
